Managed to give a definition together with the required proves! :) We use a helper function inside step, of which should be correct. Next step is to maybe prove formally that it is still the same function.

coq/SInc.v
@@ -13,284 +13,154 @@ Open Scope nat_scope.
 
 Import ListNotations.
 
-Fixpoint step (t : tree) (xs : list tree) (n : nat) {struct n} : list tree :=
-    match xs,n with
-    | nil,_       => [t]
-    | _, 0        => []
-    | u :: nil, _ =>
-        match nat_compare (ht t) (ht u) with
-        | Lt => t :: u :: nil
-        | _  => (join t u) :: nil
-        end
-    | u :: v :: ts, S n2 =>
-        match nat_compare (ht t) (ht u) with
-        | Lt => t :: u :: v :: ts
-        | _  =>
-            match nat_compare (ht t) (ht v) with
-            | Lt => step (join t u) (v :: ts) (n2)
-            | _  => step t (step (join u v) ts n2) (n2)
-            end
-        end
-    end.
-
 Inductive s_inc : (list tree) -> Prop :=
   | s_inc_nil  : s_inc nil
   | s_inc_sin  : forall (x : tree), s_inc (x :: nil)
   | s_inc_two  : forall (x y : tree), ht x < ht y -> s_inc (x :: y :: nil)
   | s_inc_cons : forall (x y : tree) (ys : list tree), ht x < ht y /\ s_inc (y :: ys) -> s_inc (x :: y :: ys).
 
+Fixpoint join_until_smaller (t : tree) (ts : list tree) :=
+  match ts with
+  | nil => [t]
+  | x :: xs => 
+    match nat_compare (ht t) (ht x) with
+    | Eq => join_until_smaller (join t x) xs
+    | Lt => t :: x :: xs
+    | Gt => join_until_smaller (join t x) xs
+    end
+  end.
 
-Theorem s_trans : forall (n m : nat),
-  S n = S m -> n = m.
+Theorem join_until_smaller_produces : forall (ts : list tree) (t : tree),
+  join_until_smaller t ts <> [].
 Proof.
-Admitted.
-
-Theorem step_bigger_inc : forall (t u : tree) (ts : list tree),
-  s_inc (u :: ts) -> ht t >= ht u -> s_inc (step t (u :: ts) (length (u :: ts))). 
-Proof.
- intros t u ts Sinc t_ge_u.
-Admitted.
-
-Theorem tuvts_step : forall (t u v : tree) (ts : list tree),
-  ht t < ht u -> step t (u :: v :: ts) (length (u :: v :: ts)) = t :: u :: v :: ts.
-Proof.
-  intros t u v ts t_lt_u.
-  simpl. remember (nat_compare (ht t) (ht u)) as H. destruct H. 
-    Focus 2. reflexivity. 
-    contradict t_lt_u. apply not_eq_r. apply eq_ge. assumption.
-    contradict t_lt_u. apply not_eq_r. apply gt_ge. assumption.
+  induction ts. simpl. intros t contra. inversion contra.
+  intros t. remember (nat_compare (ht t) (ht a)) as R. destruct R.
+    simpl. rewrite <- HeqR. apply IHts.
+    simpl. rewrite <- HeqR. intros contra. inversion contra. 
+    simpl. rewrite <- HeqR. apply IHts.
 Qed.
 
-Theorem step_jointuv : forall (t u v : tree) (ts : list tree), (* we need additional knowledge, about join t u *)
-  ht t >= ht u -> ht t < ht v -> step (join t u) (v :: ts) (length (v :: ts)) = join t u :: v :: ts.
+Theorem join_until_smaller_inc : forall (ts : list tree) (t : tree),
+  s_inc ts -> s_inc (join_until_smaller t ts).
 Proof.
-  intros t u v ts t_ge_u t_lt_v.
-  destruct ts. simpl. remember (nat_compare (max (ht t) (ht u) + 1) (ht v)) as R. destruct R.
-    
-  
-    (* step *) Focus 2. simpl.
-    remember (nat_compare (max (ht t) (ht u) + 1) (ht v)) as RM. destruct RM.
-      remember (nat_compare (max (ht t) (ht u) + 1) (ht t0)) as R2. destruct R2. simpl. 
-        destruct ts. 
-          remember (nat_compare (max (ht t) (ht u) + 1) (ht (join v t0))) as R3. destruct R3.
-            
-        remember (nat_compare (ht t) (ht v)) as R3. destruct R3.
-          contradict t_lt_v. apply not_eq_r. apply eq_ge. assumption. simpl.
-          unfold step. simpl.
-(* how to unfold properly? *)
-Admitted.
-
-Theorem step_tjoinuv : forall (t u v : tree) (ts : list tree) (H3 : nat),
-  ht t >= ht u -> ht t >= ht v -> ht t < ht (join u v) -> step t (step (join u v) ts (length (v :: ts))) (length (v :: ts)) = t :: (join u v) :: ts.
-Proof.
-Admitted.
-
-Theorem step_jointjoinuv : forall (t u v : tree) (ts : list tree) (H3 : nat),
-  ht t >= ht u -> ht t >= ht v -> ht t >= ht (join u v) -> step t (step (join u v) ts (length (v :: ts))) (length (v :: ts)) = join t (join u v) :: ts.
-Proof.
-Admitted.
-
-Theorem jtuvts_step : forall (t u v : tree) (ts : list tree),
-  ht t >= ht u -> ht t < ht v -> step t (u :: v :: ts) (length (u :: v :: ts)) = join t u :: v :: ts.
-Proof.
-  intros t u v ts t_ge_u t_lt_v.
-  remember (length (u :: v :: ts)) as H3. destruct H3. simpl in HeqH3. inversion HeqH3. simpl.
-    remember (nat_compare (ht t) (ht u)) as H. destruct H. simpl.
-      remember (nat_compare (ht t) (ht v)) as H2. destruct H2.
-        contradict t_lt_v. apply not_eq_r. apply eq_ge. assumption. 
-        Focus 2. contradict t_lt_v. apply not_eq_r. apply gt_ge. assumption.
-        Focus 2. contradict t_ge_u. apply not_ge_r. apply nat_compare_lt. symmetry. assumption.
-        Focus 2. remember (nat_compare (ht t) (ht v)) as H2. destruct H2.
-          contradict t_lt_v. apply not_eq_r. apply eq_ge. assumption.
-          Focus 2. contradict t_lt_v. apply not_eq_r. apply gt_ge. assumption.
-          apply step_jointuv. assumption. assumption. simpl in *. apply s_trans. assumption.
-        apply step_jointuv. assumption. assumption. simpl in *. apply s_trans. assumption.
+  induction ts. intros t s_inc_nil. simpl. apply s_inc_sin.
+  intros t s_inc_ats. remember (nat_compare (ht t) (ht a)) as R. destruct R.
+    simpl. rewrite <- HeqR. apply IHts. inversion s_inc_ats. apply s_inc_nil. apply s_inc_sin. destruct H0. assumption. 
+    simpl. rewrite <- HeqR. apply s_inc_cons. split. apply nat_compare_lt. symmetry. assumption. assumption.
+    simpl. rewrite <- HeqR. apply IHts. inversion s_inc_ats. apply s_inc_nil. apply s_inc_sin. destruct H0. assumption. 
 Qed.
 
-Theorem tjuvts_step : forall (t u v : tree) (ts : list tree),
-  ht t >= ht u -> ht t >= ht v -> ht t < ht (join u v) -> step t (u :: v :: ts) (length (u :: v :: ts)) = t :: (join u v) :: ts.
-Proof.
-  intros t u v ts t_ge_u t_ge_v t_lt_juv. 
-  remember (length (u :: v :: ts)) as H3. destruct H3. simpl in HeqH3. inversion HeqH3. simpl.
-    remember (nat_compare (ht t) (ht u)) as H. destruct H. simpl.
-      remember (nat_compare (ht t) (ht v)) as H2. destruct H2.
-        replace (H3) with (length (v :: ts)). apply step_tjoinuv. apply H3. assumption. assumption. assumption. simpl in *. apply s_trans in HeqH3. symmetry. assumption.
-        contradict t_ge_v. apply lt_not_le. apply nat_compare_lt. symmetry. assumption.
-        replace (H3) with (length (v :: ts)). apply step_tjoinuv. apply H3. assumption. assumption. assumption. simpl in *. apply s_trans in HeqH3. symmetry. assumption.
-        contradict t_ge_u. apply lt_not_le. apply nat_compare_lt. symmetry. assumption.
-        remember (nat_compare (ht t) (ht v)) as R3. destruct R3.
-          replace (H3) with (length (v :: ts)). apply step_tjoinuv. apply H3. assumption. assumption. assumption. simpl in *. apply s_trans in HeqH3. symmetry. assumption.
-          contradict t_ge_v. apply lt_not_le. apply nat_compare_lt. symmetry. assumption.
-          replace (H3) with (length (v :: ts)). apply step_tjoinuv. apply H3. assumption. assumption. assumption. simpl in *. apply s_trans in HeqH3. symmetry. assumption.
+Fixpoint step (t : tree) (xs : list tree) : list tree :=
+    match xs with
+    | nil  => [t]
+    | u :: vs =>
+      match vs with 
+        | nil => 
+          match nat_compare (ht t) (ht u) with
+          | Lt => t :: u :: nil
+          | _  => (join t u) :: nil
+          end
+        | v :: ts =>
+          match nat_compare (ht t) (ht u) with
+          | Lt => t :: u :: v :: ts
+          | _  =>
+              match nat_compare (ht t) (ht v) with
+              | Lt => step (join t u) vs
+              | _  => join_until_smaller t (join_until_smaller (join u v) ts)
+              end
+          end
+      end
+    end.
+
+
+Theorem step_not_nil : forall (xs : list tree) (t : tree),
+  step t xs <> [].
+Proof. 
+    (* match xs with*) induction xs as [|u].
+    (* | nil  => [t]*) simpl. intuition. inversion H.
+    (* | u :: vs =>*)
+      (* match vs with *) remember xs as vs. induction vs as [|v]; intros t. 
+        (* | nil => *)
+          (* match nat_compare (ht t) (ht u) with*) remember (nat_compare (ht t) (ht u)) as R1. destruct R1.
+          (* | Eq => (join t u) :: nil*) simpl. rewrite <- HeqR1. intros contra. inversion contra.
+          (* | Lt => t :: u :: nil*) simpl. rewrite <- HeqR1. intros contra. inversion contra.
+          (* | Gt => (join t u) :: nil*) simpl. rewrite <- HeqR1. intros contra. inversion contra.
+          (* end*)
+        (* | v :: ts =>*)
+         (* match nat_compare (ht t) (ht u) with *) remember (nat_compare (ht t) (ht u)) as R1. destruct R1.
+         (* | Eq => *) 
+              (* match nat_compare (ht t) (ht v) with *) remember (nat_compare (ht t) (ht v)) as R2. destruct R2.
+              (* | Eq =>  join_until_smaller t (join u v :: ts) *) unfold step. rewrite <- HeqR1. rewrite <- HeqR2. apply join_until_smaller_produces.
+              (* | Lt => step (join t u) vs *) rewrite Heqvs. simpl. rewrite <- Heqvs. rewrite <- HeqR1. rewrite <- HeqR2. apply IHxs.
+              (* | Gt =>  join_until_smaller t (join u v :: ts) *) unfold step. rewrite <- HeqR1. rewrite <- HeqR2. apply join_until_smaller_produces.
+              (* end *)
+         (* | Lt => t :: u :: v :: ts *) simpl.  rewrite <- HeqR1. intros contra. inversion contra.
+         (* | Gt => *) 
+              (* match nat_compare (ht t) (ht v) with *) remember (nat_compare (ht t) (ht v)) as R2. destruct R2.
+              (* | Eq =>  join_until_smaller t (join u v :: ts) *) unfold step. rewrite <- HeqR1. rewrite <- HeqR2. apply join_until_smaller_produces.
+              (* | Lt => step (join t u) vs *)  rewrite Heqvs. simpl. rewrite <- Heqvs. rewrite <- HeqR1. rewrite <- HeqR2. apply IHxs.
+              (* | Gt =>  join_until_smaller t (join u v :: ts) *) unfold step. rewrite <- HeqR1. rewrite <- HeqR2. apply join_until_smaller_produces.
+              (* end *)
+      (* end*)
+    (* end.*)
 Qed.
 
-Theorem jtjuvts_step : forall (t u v : tree) (ts : list tree),
-  ht t >= ht u -> ht t >= ht v -> ht t >= ht (join u v) -> step t (u :: v :: ts) (length (u :: v :: ts)) = join t (join u v) :: ts.
-Proof.
-  intros t u v ts t_ge_u t_ge_v t_ge_juv.
-  remember (length (u :: v :: ts)) as H3. destruct H3. simpl in HeqH3. inversion HeqH3. simpl.
-    remember (nat_compare (ht t) (ht u)) as H. destruct H. simpl.
-      remember (nat_compare (ht t) (ht v)) as H2. destruct H2.
-        replace (H3) with (length (v :: ts)). apply step_jointjoinuv. apply H3. assumption. assumption. assumption. simpl in *. apply s_trans in HeqH3. symmetry. assumption.
-        contradict t_ge_v. apply lt_not_le. apply nat_compare_lt. symmetry. assumption.
-        replace (H3) with (length (v :: ts)). apply step_jointjoinuv. apply H3. assumption. assumption. assumption. simpl in *. apply s_trans in HeqH3. symmetry. assumption.
-        contradict t_ge_u. apply lt_not_le. apply nat_compare_lt. symmetry. assumption.
-        remember (nat_compare (ht t) (ht v)) as R3. destruct R3.
-          replace (H3) with (length (v :: ts)). apply step_jointjoinuv. apply H3. assumption. assumption. assumption. simpl in *. apply s_trans in HeqH3. symmetry. assumption.
-          contradict t_ge_v. apply lt_not_le. apply nat_compare_lt. symmetry. assumption.
-          replace (H3) with (length (v :: ts)). apply step_jointjoinuv. apply H3. assumption. assumption. assumption. simpl in *. apply s_trans in HeqH3. symmetry. assumption.
-Qed.
-
-Theorem tuvts_inc_alt : forall (t u v : tree) (ts : list tree),
-  s_inc (u :: v :: ts) -> ht t < ht u -> s_inc (step t (u :: v :: ts) (length (u :: v :: ts))).
-Proof.
-intros t u v ts Sinc ht1.
-  remember (length (u :: v :: ts)) as R1. destruct R1. inversion HeqR1. simpl.
-    remember (nat_compare (ht t) (ht u)) as R2. destruct R2. simpl.
-      remember (nat_compare (ht t) (ht v)) as R3. destruct R3.
-        contradict ht1. apply not_eq_r. apply eq_ge. assumption.
-        contradict ht1. apply not_eq_r. apply eq_ge. assumption.
-        contradict ht1. apply not_eq_r. apply eq_ge. assumption.
-        apply s_inc_cons. split; assumption.
-        contradict ht1. apply not_eq_r. apply gt_ge. assumption.
-Qed.
-
-Theorem tuvts_inc : forall (t u v : tree) (ts : list tree),
-  s_inc (u :: v :: ts) -> ht t < ht u -> s_inc (t :: u :: v :: ts).
-Proof.
-intros t u v ts Sinc ht1. apply s_inc_cons. split.
-  assumption.
-  apply s_inc_cons. split.
-    inversion Sinc. assumption. inversion H0. assumption.
-    inversion Sinc. apply s_inc_sin. inversion H0. assumption.
-Qed.
-(*
-Theorem jtuvts_inc2 : forall (t u v : tree) (ts : list tree),
-  s_inc (u :: v :: ts) -> ht t >= ht u -> ht t < ht v -> ht (join t u) >= ht v -> s_inc (join (join t u) v :: ts).
-Proof.
-Admitted.
-
-Theorem jtuvts_inc3 : forall (t u v : tree) (ts : list tree),
-  s_inc (u :: v :: ts) -> ht t >= ht u -> ht t < ht v -> ht (join t u) < ht v -> s_inc (join t u :: v :: ts).
-Proof.
-  intros t u v ts Sinc t_ge_u t_lt_v jtu_lt_v. remember (nat_compare (ht (join t u)) (ht v)) as H. destruct H.
-    Focus 2. apply s_inc_cons. split.
-      assumption. 
-      inversion Sinc. apply s_inc_sin. destruct H0. assumption.
-    contradict jtu_lt_v. apply not_eq_r. apply eq_ge. assumption.
-    contradict jtu_lt_v. apply not_eq_r. apply gt_ge. assumption.
-Qed.
-*)
-Theorem jtuvts_inc : forall (t u v : tree) (ts : list tree),
-  s_inc (u :: v :: ts) -> ht t >= ht u -> ht t < ht v -> s_inc (step (join t u) (v :: ts) (length (v :: ts))).
-Proof.
-  intros t u v ts Sinc t_ge_u t_lt_v. 
-    induction ts. 
-    (* base *)
-      simpl. remember (nat_compare (max (ht t) (ht u) + 1) (ht v)) as R1. destruct R1.
-        apply s_inc_sin.
-        apply s_inc_two. simpl. apply nat_compare_lt. symmetry. assumption.
-        apply s_inc_sin.
-    (* step *)
-      remember (nat_compare (ht (join t u)) (ht v)) as R. destruct R.
-        Focus 2. apply tuvts_inc_alt. inversion Sinc. inversion H0. assumption. apply nat_compare_lt. symmetry. assumption.
-        apply step_bigger_inc. inversion Sinc. inversion H0. assumption. apply eq_ge. assumption.
-        apply step_bigger_inc. inversion Sinc. inversion H0. assumption. apply gt_ge. assumption.
-Qed.
-
-Theorem tjuvts_inc : forall (t u v : tree) (ts : list tree),
-  s_inc (u :: v :: ts) -> ht t >= ht u -> ht t >= ht v -> ht t < ht (join u v) ->  s_inc (t :: (join u v) :: ts).
-Proof.
-Admitted.
-
-Theorem jtjuvts_inc : forall (t u v : tree) (ts : list tree),
-  s_inc (u :: v :: ts) -> ht t >= ht u -> ht t >= ht v -> ht t >= ht (join u v) -> s_inc (join t (join u v) :: ts).
-Proof.
-Admitted.
-
-Theorem step_inc : forall (l : list tree) (t : tree),
-  s_inc l -> s_inc (step t l (length l)).
-Proof.
-  induction l. simpl. intros t Sinc. apply s_inc_sin.
-  (* step *) induction l. simpl. intros t sIncA. remember (nat_compare (ht t) (ht a)) as H. destruct H; [apply s_inc_sin | apply s_inc_two; apply nat_compare_lt; symmetry; assumption | apply s_inc_sin].
-    (* step *) intros t sInc. remember (nat_compare (ht t) (ht a)) as H. destruct H.
-        remember (nat_compare (ht t) (ht a0)) as H2. destruct H2.
-          rewrite tjuvts_step. apply tjuvts_inc. assumption. apply eq_ge. assumption. 
-                                                 apply eq_ge. assumption. simpl. unfold max. case (nat_compare (ht a) (ht a0)). 
-                                                 apply eq_ge. assumption.
-                                                 apply eq_ge. assumption.
-          rewrite jtuvts_step. apply jtuvts_inc. assumption. apply eq_ge. assumption.
-                                                 apply nat_compare_lt. symmetry. assumption.
-                                                 apply eq_ge. assumption.
-                                                 apply nat_compare_lt. symmetry. assumption.
-          rewrite jtjuvts_step. apply jtjuvts_inc. assumption. apply eq_ge. assumption.
-                                                 apply gt_ge. assumption.
-                                                 apply eq_ge. assumption.
-                                                 apply gt_ge. assumption.
-        remember (nat_compare (ht t) (ht a0)) as H2. destruct H2.
-          rewrite tuvts_step. apply tuvts_inc. assumption. apply nat_compare_lt. symmetry. assumption.
-                                                 apply nat_compare_lt. symmetry. assumption. 
-          rewrite tuvts_step. apply tuvts_inc. assumption. apply nat_compare_lt. symmetry. assumption.  
-                                                 apply nat_compare_lt. symmetry. assumption. 
-          rewrite tuvts_step. apply tuvts_inc. assumption. apply nat_compare_lt. symmetry. assumption.  
-                                                 apply nat_compare_lt. symmetry. assumption. 
-        remember (nat_compare (ht t) (ht a0)) as H2. destruct H2.
-          rewrite jtjuvts_step. apply jtjuvts_inc. assumption. apply gt_ge. assumption. 
-                                                 apply eq_ge. assumption.
-                                                 apply gt_ge. assumption.
-                                                 apply eq_ge. assumption.
-          rewrite jtuvts_step. apply jtuvts_inc. assumption. apply gt_ge. assumption.
-                                                 apply nat_compare_lt. symmetry. assumption.
-                                                 apply gt_ge. assumption.
-                                                 apply nat_compare_lt. symmetry. assumption.
-          rewrite jtjuvts_step. apply jtjuvts_inc. assumption. apply gt_ge. assumption.
-                                                 apply gt_ge. assumption.
-                                                 apply gt_ge. assumption.
-                                                 apply gt_ge. assumption.
-Qed.
-
-
-Theorem step_not_nil : forall (l : list tree) (t : tree),
-  step t l (length l) <> [].
-Proof.
-  induction l. simpl. intros t contra. inversion contra. 
- (* step *) induction l. simpl. intros t. case (nat_compare (ht t) (ht a)). intros contra. inversion contra. intros contra. inversion contra. intros contra. inversion contra. 
-   (* step *) intros t. remember (nat_compare (ht t) (ht a)) as H. destruct H.
-        remember (nat_compare (ht t) (ht a0)) as H2. destruct H2.
-          rewrite jtjuvts_step. intuition. inversion H. apply eq_ge. assumption. 
-                                                 apply eq_ge. assumption.
-          rewrite jtuvts_step. intuition. inversion H. apply eq_ge. assumption.
-                                                 apply nat_compare_lt. symmetry. assumption.
-          rewrite jtjuvts_step. intuition. inversion H. apply eq_ge. assumption.
-                                                 apply gt_ge. assumption.
-        remember (nat_compare (ht t) (ht a0)) as H2. destruct H2.
-          rewrite tuvts_step. intuition. inversion H. apply nat_compare_lt. symmetry. assumption.
-          rewrite tuvts_step. intuition. inversion H. apply nat_compare_lt. symmetry. assumption. 
-          rewrite tuvts_step. intuition. inversion H. apply nat_compare_lt. symmetry. assumption. 
-        remember (nat_compare (ht t) (ht a0)) as H2. destruct H2.
-          rewrite jtjuvts_step. intuition. inversion H. apply gt_ge. assumption. 
-                                                 apply eq_ge. assumption.
-          rewrite jtuvts_step. intuition. inversion H. apply gt_ge. assumption.
-                                                 apply nat_compare_lt. symmetry. assumption.
-          rewrite jtjuvts_step. intuition. inversion H. apply gt_ge. assumption.
-                                                 apply gt_ge. assumption.
+Theorem step_inc : forall (xs : list tree) (t : tree),
+  s_inc xs -> s_inc (step t xs).
+Proof. 
+    (* match xs with*) induction xs as [|u].
+    (* | nil  => [t]*) simpl. intuition. apply s_inc_sin.
+    (* | u :: vs =>*)
+      (* match vs with *) remember xs as vs. induction vs as [|v]; intros t H. 
+        (* | nil => *)
+          (* match nat_compare (ht t) (ht u) with*) remember (nat_compare (ht t) (ht u)) as R1. destruct R1.
+          (* | Eq => (join t u) :: nil*) simpl. rewrite <- HeqR1. apply s_inc_sin.
+          (* | Lt => t :: u :: nil*) simpl. rewrite <- HeqR1. apply s_inc_two. apply nat_compare_lt. symmetry. assumption.
+          (* | Gt => (join t u) :: nil*) simpl. rewrite <- HeqR1. apply s_inc_sin.
+          (* end*)
+        (* | v :: ts =>*)
+         (* match nat_compare (ht t) (ht u) with *) remember (nat_compare (ht t) (ht u)) as R1. destruct R1.
+         (* | Eq => *) 
+              (* match nat_compare (ht t) (ht v) with *) remember (nat_compare (ht t) (ht v)) as R2. destruct R2.
+              (* | Eq =>  join_until_smaller t (join u v :: ts) *) inversion H. contradict H1. apply not_eq_r. apply eq_ge. apply eq_nmo_mo with (n := ht t); assumption. 
+                                                                   inversion H1. contradict H4. apply not_eq_r. apply eq_ge. apply eq_nmo_mo with (n := ht t); assumption.
+              (* | Lt => step (join t u) vs *) rewrite Heqvs. simpl. rewrite <- Heqvs. rewrite <- HeqR1. rewrite <- HeqR2. apply IHxs. inversion H. apply s_inc_sin. inversion H1. assumption.
+              (* | Gt =>  join_until_smaller t (join u v :: ts) *) inversion H. contradict H1. apply not_eq_r. apply gt_ge. apply gt_nmo_mo with (n := ht t); assumption. 
+                                                                   inversion H1. contradict H4. apply not_eq_r. apply gt_ge. apply gt_nmo_mo with (n := ht t); assumption. 
+              (* end *)
+         (* | Lt => t :: u :: v :: ts *) simpl.  rewrite <- HeqR1. apply s_inc_cons. split. apply nat_compare_lt. symmetry. assumption. assumption.
+         (* | Gt => *) 
+              (* match nat_compare (ht t) (ht v) with *) remember (nat_compare (ht t) (ht v)) as R2. destruct R2.
+              (* | Eq =>  join_until_smaller t (join u v :: ts) *) simpl. rewrite <- HeqR1. rewrite <- HeqR2. remember (nat_compare (ht t) (max (ht u) (ht v) + 1)) as R3. destruct R3.
+                                                                     apply join_until_smaller_inc. apply join_until_smaller_inc. inversion H. apply s_inc_nil. inversion H1. inversion H5. apply s_inc_nil. apply s_inc_sin. inversion H7. assumption.
+                                                                     apply join_until_smaller_inc. apply join_until_smaller_inc. inversion H. apply s_inc_nil. inversion H1. inversion H5. apply s_inc_nil. apply s_inc_sin. inversion H7. assumption.
+                                                                     apply join_until_smaller_inc. apply join_until_smaller_inc. inversion H. apply s_inc_nil. inversion H1. inversion H5. apply s_inc_nil. apply s_inc_sin. inversion H7. assumption.
+              (* | Lt => step (join t u) vs *)  rewrite Heqvs. simpl. rewrite <- Heqvs. rewrite <- HeqR1. rewrite <- HeqR2. apply IHxs. inversion H. apply s_inc_sin. inversion H1. assumption. 
+              (* | Gt =>  join_until_smaller t (join u v :: ts) *)  simpl. rewrite <- HeqR1. rewrite <- HeqR2. remember (nat_compare (ht t) (max (ht u) (ht v) + 1)) as R3. destruct R3.
+                                                                     apply join_until_smaller_inc. apply join_until_smaller_inc. inversion H. apply s_inc_nil. inversion H1. inversion H5. apply s_inc_nil. apply s_inc_sin. inversion H7. assumption.
+                                                                     apply join_until_smaller_inc. apply join_until_smaller_inc. inversion H. apply s_inc_nil. inversion H1. inversion H5. apply s_inc_nil. apply s_inc_sin. inversion H7. assumption.
+                                                                     apply join_until_smaller_inc. apply join_until_smaller_inc. inversion H. apply s_inc_nil. inversion H1. inversion H5. apply s_inc_nil. apply s_inc_sin. inversion H7. assumption.
+              (* end *)
+      (* end*)
+    (* end.*)
 Qed.
 
 Theorem fold_right_not_nil : forall (l : list tree),
-  l <> [] -> fold_right (fun (a : tree) (xs : list tree) => step a xs (length xs)) [] l <> [].
+  l <> [] -> fold_right (fun (a : tree) (xs : list tree) => step a xs) [] l <> [].
 Proof.
   induction l. intros LNNil. simpl. assumption.
   (* step *) intros alNNil. simpl. apply step_not_nil.
 Qed.
 
 Theorem fold_step_not_nil : forall (l : list tree),
-  l <> nil -> (fold_right (fun (a : tree) (xs : list tree) => step a xs (length xs)) nil l) <> nil.
+  l <> nil -> (fold_right (fun (a : tree) (xs : list tree) => step a xs) nil l) <> nil.
 Proof.
   intros l NNil. apply fold_right_not_nil. assumption.
 Qed.
 
 Theorem fold_right_step : forall (l : list tree),
-  s_inc (fold_right (fun (a : tree) (xs : list tree) => step a xs (length xs)) nil l).
+  s_inc (fold_right (fun (a : tree) (xs : list tree) => step a xs) nil l).
 Proof.
   induction l as [|l']. simpl. apply s_inc_nil. simpl. apply step_inc. assumption.
 Qed.
+  
