coq/Helpers.v
@@ -25,3 +25,23 @@ Theorem not_ge_r : forall (n m : nat),
   n < m -> ~ n >= m.
 Proof.
 Admitted.
+
+Theorem eq_nmo_mo : forall (n m o : nat),
+  Eq = nat_compare n m -> Eq = nat_compare n o -> Eq = nat_compare m o.
+Proof.
+  intros n m o H1 H2. 
+    assert (A1 : n = m). apply nat_compare_eq. symmetry. assumption. 
+    assert (A2 : n = o). apply nat_compare_eq. symmetry. assumption. 
+    rewrite A1 in H2. 
+    assumption.
+Qed.
+
+Theorem gt_nmo_mo : forall (n m o : nat),
+  Eq = nat_compare n m -> Gt = nat_compare n o -> Gt = nat_compare m o.
+Proof.
+  intros n m o H1 H2. 
+    assert (A1 : n = m). apply nat_compare_eq. symmetry. assumption. 
+    assert (A2 : n > o). apply nat_compare_gt. symmetry. assumption. 
+    rewrite A1 in H2. 
+    assumption.
+Qed.
